bedrock2/src/bedrock2/BasicC32Semantics.v
@@ -4,22 +4,24 @@ Require coqutil.Datatypes.String coqutil.Map.SortedList coqutil.Map.SortedListSt
 Require Import coqutil.Word.Interface coqutil.Word.Bitwidth32 coqutil.Map.SortedListWord.
 Require coqutil.Word.Naive.
 
-Instance parameters : parameters :=
-  let word := Naive.word32 in
-  {|
-  width := 32;
-  mem := SortedListWord.map _ _;
-  locals := SortedListString.map _;
-  env := SortedListString.map _;
-  ext_spec := fun _ _ _ _ _ => False;
-|}.
+Instance word: word.word 32 := Naive.word32.
+Instance mem: Interface.map.map word Byte.byte := SortedListWord.map _ _.
+Instance locals: Interface.map.map String.string word := SortedListString.map _.
+Instance env: Interface.map.map String.string (list String.string * list String.string * cmd) :=
+  SortedListString.map _.
+Instance ext_spec: ExtSpec := fun _ _ _ _ _ => False.
 
-Global Instance ok trace m0 act args :
+Arguments word: simpl never.
+Arguments mem: simpl never.
+Arguments locals: simpl never.
+Arguments env: simpl never.
+
+Instance weaken_ext_spec trace m0 act args :
   Morphisms.Proper
     (Morphisms.respectful
        (Morphisms.pointwise_relation Interface.map.rep
-          (Morphisms.pointwise_relation (list Semantics.word) Basics.impl))
-       Basics.impl) (Semantics.ext_spec trace m0 act args).
+          (Morphisms.pointwise_relation (list word) Basics.impl))
+       Basics.impl) (ext_spec trace m0 act args).
 Proof.
   cbn in *.
   unfold Morphisms.Proper, Morphisms.respectful, Morphisms.pointwise_relation, Basics.impl.
@@ -28,29 +30,16 @@ Proof.
 Qed.
 
 Instance localsok: coqutil.Map.Interface.map.ok locals := SortedListString.ok _.
+Instance envok: coqutil.Map.Interface.map.ok env := SortedListString.ok _.
 Instance mapok: coqutil.Map.Interface.map.ok mem := SortedListWord.ok Naive.word32 _.
-Instance wordok: coqutil.Word.Interface.word.ok Semantics.word := Naive.word32_ok.
-Add Ring wring : (Properties.word.ring_theory (word := Semantics.word))
+Instance wordok: coqutil.Word.Interface.word.ok word := Naive.word32_ok.
+Add Ring wring : (Properties.word.ring_theory (word := word))
       (preprocess [autorewrite with rew_word_morphism],
-       morphism (Properties.word.ring_morph (word := Semantics.word)),
+       morphism (Properties.word.ring_morph (word := word)),
        constants [Properties.word_cst]).
 
-Global Instance ext_spec_ok trace m0 act args :
-  Morphisms.Proper
-    (Morphisms.respectful
-       (Morphisms.pointwise_relation Interface.map.rep
-          (Morphisms.pointwise_relation (list Semantics.word) Basics.impl))
-       Basics.impl) (Semantics.ext_spec trace m0 act args).
+Instance ext_spec_ok : ext_spec.ok ext_spec.
 Proof.
-  cbn in *.
-  unfold Morphisms.Proper, Morphisms.respectful, Morphisms.pointwise_relation, Basics.impl.
-  intros.
-  assumption.
-Qed.
-
-Instance parameters_ok : parameters_ok parameters.
-  constructor; intros; try typeclasses eauto.
-  - unfold env, parameters. exact (SortedListString.ok _).
-  - constructor.
-    all: try typeclasses eauto; intros; cbn in *; contradiction.
+  constructor; intros; try contradiction.
+  apply weaken_ext_spec.
 Qed.
