bedrock2/src/bedrock2Examples/ARPResponder.v
@@ -1,14 +1,12 @@
 Require Import bedrock2.Syntax.
-Require Import bedrock2.NotationsCustomEntry coqutil.Z.HexNotation.
+Require Import bedrock2.NotationsCustomEntry.
 Require Import bedrock2.FE310CSemantics.
 
-Section WithParameters.
-  Context {p : FE310CSemantics.parameters}.
-  Import Syntax BinInt String List.ListNotations ZArith.
-  Local Open Scope string_scope. Local Open Scope Z_scope. Local Open Scope list_scope.
-  Local Coercion expr.literal : Z >-> expr.
-  Local Coercion expr.var : String.string >-> expr.
-  Local Coercion name_of_func (f : function) : String.string := fst f.
+Import Syntax BinInt String List.ListNotations ZArith.
+Local Open Scope string_scope. Local Open Scope Z_scope. Local Open Scope list_scope.
+Local Coercion expr.literal : Z >-> expr.
+Local Coercion expr.var : String.string >-> expr.
+Local Coercion name_of_func (f : function) : String.string := fst f.
 
 Definition arp : bedrock_func :=
     let ethbuf : String.string := "ethbuf" in
@@ -18,7 +16,7 @@ Definition arp : bedrock_func :=
     require ( coq:(14+27) < len ) else { /*skip*/ };
     require ( (load1(ethbuf+coq:(14+0))== coq:(0))
             & (load1(ethbuf+coq:(14+1)) == coq:(1))
-            & (load1(ethbuf+coq:(14+2)) == coq:(Ox"08"))
+            & (load1(ethbuf+coq:(14+2)) == coq:(0x08))
             & (load1(ethbuf+coq:(14+3)) == coq:(0))
             & (load1(ethbuf+coq:(14+4)) == coq:(6))
             & (load1(ethbuf+coq:(14+5)) == coq:(4))
@@ -51,24 +49,24 @@ Definition arp : bedrock_func :=
     store1(ethbuf+coq:(5), load1(ethbuf+coq:(14+8+5)));
 
     (* src := me *)
-    store1(ethbuf+coq:(14+8  ), coq:(Ox"f0"));
-    store1(ethbuf+coq:(14+8+1), coq:(Ox"f1"));
-    store1(ethbuf+coq:(14+8+2), coq:(Ox"f2"));
-    store1(ethbuf+coq:(14+8+3), coq:(Ox"f3"));
-    store1(ethbuf+coq:(14+8+4), coq:(Ox"f4"));
-    store1(ethbuf+coq:(14+8+5), coq:(Ox"f5"));
+    store1(ethbuf+coq:(14+8  ), coq:(0xf0));
+    store1(ethbuf+coq:(14+8+1), coq:(0xf1));
+    store1(ethbuf+coq:(14+8+2), coq:(0xf2));
+    store1(ethbuf+coq:(14+8+3), coq:(0xf3));
+    store1(ethbuf+coq:(14+8+4), coq:(0xf4));
+    store1(ethbuf+coq:(14+8+5), coq:(0xf5));
     store1(ethbuf+coq:(14+8+6), coq:( 10));
     store1(ethbuf+coq:(14+8+7), coq:(155));
     store1(ethbuf+coq:(14+8+8), coq:(  5));
     store1(ethbuf+coq:(14+8+9), coq:(  1));
 
     (* eth_src = me *)
-    store1(ethbuf+coq:(6+0), coq:(Ox"f0"));
-    store1(ethbuf+coq:(6+1), coq:(Ox"f1"));
-    store1(ethbuf+coq:(6+2), coq:(Ox"f2"));
-    store1(ethbuf+coq:(6+3), coq:(Ox"f3"));
-    store1(ethbuf+coq:(6+4), coq:(Ox"f4"));
-    store1(ethbuf+coq:(6+5), coq:(Ox"f5"));
+    store1(ethbuf+coq:(6+0), coq:(0xf0));
+    store1(ethbuf+coq:(6+1), coq:(0xf1));
+    store1(ethbuf+coq:(6+2), coq:(0xf2));
+    store1(ethbuf+coq:(6+3), coq:(0xf3));
+    store1(ethbuf+coq:(6+4), coq:(0xf4));
+    store1(ethbuf+coq:(6+5), coq:(0xf5));
 
     /*skip*/
 ))).
@@ -89,10 +87,10 @@ Definition ethernet : bedrock_func :=
   ("ethernet", ((buf::len::nil), @nil String.string, bedrock_func_body:(
     require (coq:(14) < len) else { /*skip*/ } ;
     ethertype = (load1(buf + coq:(12)) << coq:(8)) | (load1(buf + coq:(13)));
-    require (coq:(Ox"600"-1) < ethertype) else { /*skip*/ };
-    if (ethertype == coq:(Ox"0800")) {
+    require (coq:(0x600-1) < ethertype) else { /*skip*/ };
+    if (ethertype == coq:(0x0800)) {
       ipv4(buf+coq:(14), len-coq:(14))
-    } else if (ethertype == coq:(Ox"0806")) {
+    } else if (ethertype == coq:(0x0806)) {
       arp(buf, len)
     }
 ))).
@@ -106,4 +104,3 @@ Goal True.
         *)
   .
 Abort.
-End WithParameters.
