bedrock2/src/bedrock2Examples/memmove.v
@@ -4,7 +4,8 @@ Import Syntax Syntax.Coercions BinInt String List List.ListNotations.
 Local Open Scope string_scope. Local Open Scope Z_scope. Local Open Scope list_scope.
 
 Require Import bedrock2.WeakestPrecondition bedrock2.Semantics bedrock2.ProgramLogic.
-Require Import coqutil.Word.Interface coqutil.Map.Interface bedrock2.Map.SeparationLogic.
+Require Import coqutil.Word.Interface coqutil.Word.Bitwidth.
+Require Import coqutil.Map.Interface bedrock2.Map.SeparationLogic.
 
 (*Require Import bedrock2.ptsto_bytes.*)
 Require Import coqutil.Map.OfListWord.
@@ -12,12 +13,15 @@ Local Notation "xs $@ a" := (map.of_list_word_at a xs) (at level 10, format "xs 
 Local Notation "m =* P" := ((P%sep) m) (at level 70, only parsing) (* experiment*).
 
 Section WithParameters.
-  Context {p : Semantics.parameters}.
+  Context {width} {BW: Bitwidth width}.
+  Context {word: word.word width} {mem: map.map word Byte.byte} {locals: map.map String.string word}.
+  Context {ext_spec: ExtSpec}.
+  Context {word_ok: word.ok word} {mem_ok: map.ok mem}.
   Import ProgramLogic.Coercions.
 
 
   Instance spec_of_memmove : spec_of "memmove" :=
-    fnspec! "memmove" dst src (n : Semantics.word) / d s R Rs,
+    fnspec! "memmove" dst src (n : word) / d s R Rs,
     { requires t m := m =* s$@src * Rs /\ m =* d$@dst * R /\
       length s = n :> Z /\ length d = n :> Z /\ n < 2^(width-1);
       ensures t' m' := t=t' /\ sep (eq(s$@dst)) R m }.
